WIP: sched

src/Concurrency.v
@@ -13,33 +13,45 @@ From Fairness Require Import Mod.
 
 Set Implicit Arguments.
 
-Section YIELD.
+Section SCHEDULE.
 
-  Variable State: Type.
+  Context {Ident: ID}.
+  (* Variable State: Type. *)
 
-  Variant cE: Type -> Type :=
-    | Yield (st: State): cE State
-  .
+  (* Variant cE: Type -> Type := *)
+  (*   | Yield (st: State): cE State *)
+  (* . *)
 
-  Definition Es := cE+'eventE.
+  (* Definition Es := cE +' eventE. *)
+  Definition Es := (@eventE (id_sum tids Ident)) +' cE.
 
-  Definition thread {R} := stateT State (itree Es) R.
-  Definition threads {R} := id -> @thread R.
+  (* Definition thread {R} := stateT State (itree Es) R. *)
+  Definition thread {R} := itree Es R.
+  Definition threads {R} := tids.(id) -> @thread R.
 
-  Definition update_threads {R} (tid: id) (k: thread) (ts: threads) : @threads R :=
-    fun t => if (Tid_eq_dec tid t) then k else (ts t).
+  Definition update_threads {R} (tid: tids.(id)) (th: thread) (ths: threads) : @threads R :=
+    fun t => if (tid_dec tid t) then th else (ths t).
 
-  Definition interp_yield {R}:
-    ((@threads R) * ((id * itree Es (State * R)) + State)) -> itree eventE void.
+  Definition sum_fmap_l {A B: ID} (fm: @fmap A): @fmap (id_sum A B) :=
+    fun sa => match sa with | inl a => (fm a) | inr _ => Flag.emp end.
+
+  Definition sum_fmap_r {A B: ID} (fm: @fmap B): @fmap (id_sum A B) :=
+    fun sb => match sb with | inl _ => Flag.emp | inr b => (fm b) end.
+
+  Definition interp_concurrent {R}:
+    ((@threads R) * (tids.(id) * itree Es R)) -> itree (@eventE (id_sum tids Ident)) unit.
   Proof.
-    eapply ITree.iter. intros [threads [[tid itr]|]].
-    - destruct (observe itr).
-      + exact (Ret (inl (threads, inr (fst r)))).
-      + exact (Ret (inl (threads, inl (tid, t)))).
-      + destruct e.
-        * destruct c. exact (Ret (inl (update_threads tid k threads, inr st))).
-        * exact (Vis e (fun x => Ret (inl (threads, inl (tid, k x))))).
-    - exact (Vis (Choose id) (fun tid => Ret (inl (threads, inl (tid, (threads tid s)))))).
+    eapply ITree.iter. intros [threads [tid itr]].
+    destruct (observe itr).
+      - exact (Ret (inl (threads, (tid, Ret r)))).
+      - exact (Ret (inl (threads, (tid, t)))).
+      - destruct e.
+        + exact (Vis e (fun x => Ret (inl (threads, (tid, k x))))).
+        + destruct c.
+          * exact (Vis (Choose tids.(id))
+                       (fun t => Vis (Fair (sum_fmap_l (thread_fmap t)))
+                                  (fun _ => Ret (inl (update_threads t (k tt) threads, (t, k tt)))))).
+          * exact (Ret (inl (threads, (tid, k tid)))).
   Defined.
 
   (* Definition interp_yield {R}: *)
@@ -68,6 +80,8 @@ Section YIELD.
   Proof.
     apply bisim_is_eq. eapply unfold_iter.
   Qed.
+
+  (*TODO*)
 
   Lemma interp_yield_ret R (threads: @threads R) tid st r
     :
@@ -155,4 +169,91 @@ Section YIELD.
   (*     = *)
   (*     ?? *)
   (* . *)
-End YIELD.
+
+  (* Lemma interp_yield_ret R (threads: @threads R) tid st r *)
+  (*   : *)
+  (*   interp_yield (threads, inl (tid, Ret (st, r))) = tau;; interp_yield (threads, inr st). *)
+  (* Proof. *)
+  (*   unfold interp_yield. rewrite unfold_iter. ss. grind. *)
+  (* Qed. *)
+
+  (* Lemma interp_yield_tau R (threads: @threads R) tid itr *)
+  (*   : *)
+  (*   interp_yield (threads, inl (tid, tau;; itr)) = tau;; interp_yield (threads, inl (tid, itr)). *)
+  (* Proof. *)
+  (*   unfold interp_yield. rewrite unfold_iter. ss. grind. *)
+  (* Qed. *)
+
+  (* Lemma interp_yield_yield_vis R (threads: @threads R) tid st k *)
+  (*   : *)
+  (*   interp_yield (threads, inl (tid, Vis (Yield st|)%sum k)) *)
+  (*   = *)
+  (*     tau;; interp_yield (update_threads tid k threads, inr st). *)
+  (* Proof. *)
+  (*   unfold interp_yield. rewrite unfold_iter. ss. grind. *)
+  (* Qed. *)
+
+  (* Lemma interp_yield_yield R (threads: @threads R) tid st k *)
+  (*   : *)
+  (*   interp_yield (threads, inl (tid, trigger (Yield st|)%sum >>= k)) *)
+  (*   = *)
+  (*     tau;; interp_yield (update_threads tid k threads, inr st). *)
+  (* Proof. *)
+  (*   rewrite bind_trigger. apply interp_yield_yield_vis. *)
+  (* Qed. *)
+
+  (* Lemma interp_yield_vis R (threads: @threads R) tid X (e: eventE X) k *)
+  (*   : *)
+  (*   interp_yield (threads, inl (tid, Vis (|e)%sum k)) *)
+  (*   = *)
+  (*     Vis e (fun x => tau;; interp_yield (threads, inl (tid, k x))). *)
+  (* Proof. *)
+  (*   unfold interp_yield. rewrite unfold_iter. ss. rewrite bind_vis. *)
+  (*   apply observe_eta. ss. f_equal. extensionality x. *)
+  (*   rewrite bind_ret_l. reflexivity. *)
+  (* Qed. *)
+
+  (* Lemma interp_yield_trigger R (threads: @threads R) tid X (e: eventE X) k *)
+  (*   : *)
+  (*   interp_yield (threads, inl (tid, trigger (|e)%sum >>= k)) *)
+  (*   = *)
+  (*     x <- trigger e;; tau;; interp_yield (threads, inl (tid, k x)). *)
+  (* Proof. *)
+  (*   rewrite ! bind_trigger. apply interp_yield_vis. *)
+  (* Qed. *)
+
+  (* Lemma interp_yield_pick_vis R (threads: @threads R) st *)
+  (*   : *)
+  (*   interp_yield (threads, inr st) *)
+  (*   = *)
+  (*     Vis (Choose id) (fun tid => tau;; interp_yield (threads, inl (tid, (threads tid st)))). *)
+  (* (* Vis (Choose _ Tid) (fun tid => *) *)
+  (* (*                     '(itr, threads) <- unwrapN (alist_pop tid threads);; *) *)
+  (* (*                     tau;; interp_yield (threads, inl (tid, itr st))). *) *)
+  (* Proof. *)
+  (*   unfold interp_yield. rewrite unfold_iter. rewrite bind_vis. *)
+  (*   apply observe_eta. ss. f_equal. extensionality x. *)
+  (*   grind. *)
+  (*   (* rewrite bind_bind. f_equal. extensionality r. destruct r; ss. *) *)
+  (*   (* rewrite bind_ret_l. refl. *) *)
+  (* Qed. *)
+
+  (* Lemma interp_yield_pick R (threads: @threads R) st *)
+  (*   : *)
+  (*   interp_yield (threads, inr st) *)
+  (*   = *)
+  (*     tid <- trigger (Choose id);; *)
+  (*     tau;; interp_yield (threads, inl (tid, threads tid st)). *)
+  (* (* '(itr, threads) <- unwrapN (alist_pop tid threads);; *) *)
+  (* (* tau;; interp_yield (threads, inl (tid, itr st)). *) *)
+  (* Proof. *)
+  (*   rewrite bind_trigger. apply interp_yield_pick_vis. *)
+  (* Qed. *)
+
+  (* (* Lemma interp_yield_bind R (threads: alist Tid (stateT State (itree Es) R)) tid A (itr: itree Es A) ktr *) *)
+  (* (*   : *) *)
+  (* (*     interp_yield (threads, inl (tid, itr >>= ktr)) *) *)
+  (* (*     = *) *)
+  (* (*     ?? *) *)
+  (* (* . *) *)
+End SCHEDULE.
